\documentclass[12pt, letterpaper]{article}
\usepackage{amsthm,amssymb}
\usepackage{mathtext}
\usepackage[T1]{fontenc}
\usepackage[utf8]{inputenc}
\usepackage{pgfplots}
\pgfplotsset{compat=1.9}
\usepackage[english,russian]{babel}
\title{Лабораторная работа минимум на отл 10!}
\author{Рогов Анатолий Б01-406}
\date{\today}
\begin{document}
\maketitle
\newpage
\section{Исходная функция}
\centering
$f(x) = ({2}\cdot{(e^{({x}\cdot{2})})})$\\
\begin{figure}[h]
\centering
\begin{tikzpicture}
\begin{axis} [
	legend pos = north west,
	xlabel = {$x$},
	ylabel = {$f$},
	xmin = -6,
	xmax = 6,
	restrict y to domain=-30:30,
	grid = major,
	enlargelimits=true,
]
\legend{
	$({2}\cdot{(e^{({x}\cdot{2})})})$
}
\addplot[blue, samples=750]{(((2))*((exp((((x))*((2)))))))};
\end{axis}
\end{tikzpicture}
\caption{График функции}
\end{figure}
\newpage
\section{Дифференцирование}
$f^{(1)}(x) = ({2}\cdot{({(e^{({x}\cdot{2})})}\cdot{2})})$\\
$f^{(2)}(x) = ({2}\cdot{({({(e^{({x}\cdot{2})})}\cdot{2})}\cdot{2})})$\\
$f^{(3)}(x) = ({2}\cdot{({({({(e^{({x}\cdot{2})})}\cdot{2})}\cdot{2})}\cdot{2})})$\\
$f^{(4)}(x) = ({2}\cdot{({({({({(e^{({x}\cdot{2})})}\cdot{2})}\cdot{2})}\cdot{2})}\cdot{2})})$\\
$f^{(5)}(x) = ({2}\cdot{({({({({({(e^{({x}\cdot{2})})}\cdot{2})}\cdot{2})}\cdot{2})}\cdot{2})}\cdot{2})})$\\
$f^{(6)}(x) = ({2}\cdot{({({({({({({(e^{({x}\cdot{2})})}\cdot{2})}\cdot{2})}\cdot{2})}\cdot{2})}\cdot{2})}\cdot{2})})$\\
$f^{(7)}(x) = ({2}\cdot{({({({({({({({(e^{({x}\cdot{2})})}\cdot{2})}\cdot{2})}\cdot{2})}\cdot{2})}\cdot{2})}\cdot{2})}\cdot{2})})$\\
$f^{(8)}(x) = ({2}\cdot{({({({({({({({({(e^{({x}\cdot{2})})}\cdot{2})}\cdot{2})}\cdot{2})}\cdot{2})}\cdot{2})}\cdot{2})}\cdot{2})}\cdot{2})})$\\
$f^{(9)}(x) = ({2}\cdot{({({({({({({({({({(e^{({x}\cdot{2})})}\cdot{2})}\cdot{2})}\cdot{2})}\cdot{2})}\cdot{2})}\cdot{2})}\cdot{2})}\cdot{2})}\cdot{2})})$\\
$f^{(10)}(x) = ({2}\cdot{({({({({({({({({({({(e^{({x}\cdot{2})})}\cdot{2})}\cdot{2})}\cdot{2})}\cdot{2})}\cdot{2})}\cdot{2})}\cdot{2})}\cdot{2})}\cdot{2})}\cdot{2})})$\\
$f^{(11)}(x) = ({2}\cdot{({({({({({({({({({({({(e^{({x}\cdot{2})})}\cdot{2})}\cdot{2})}\cdot{2})}\cdot{2})}\cdot{2})}\cdot{2})}\cdot{2})}\cdot{2})}\cdot{2})}\cdot{2})}\cdot{2})})$\\
\end{document}
